matching-logic/src/Syntax.v
@@ -28,8 +28,6 @@ From MatchingLogic Require Export
 
 Import MatchingLogic.Substitution.Notations.
 
-Definition Theory {Σ : Signature} := propset Pattern.
-
 Close Scope boolean_if_scope.
 
 Section syntax.
@@ -735,214 +733,10 @@ Section with_signature.
       reflexivity.
   Qed.
 
+  Locate svar_quantify.
+  
 
-  Lemma Private_no_negative_occurrence_svar_quantify ϕ level X:
-    (
-      no_negative_occurrence_db_b level ϕ = true ->
-      svar_has_negative_occurrence X ϕ = false ->
-      no_negative_occurrence_db_b level (ϕ^{{svar: X ↦ level}}) = true
-    )
-    /\
-    (
-      no_positive_occurrence_db_b level ϕ = true ->
-      svar_has_positive_occurrence X ϕ = false ->
-      no_positive_occurrence_db_b level (ϕ^{{svar: X ↦ level}}) = true
-    ).
-  Proof.
-    move: level.
-    induction ϕ; intros level; split; intros HnoX Hnolevel; cbn in *; auto.
-    - case_match; reflexivity.
-    - case_match; cbn. 2: reflexivity. congruence.
-    - apply orb_false_iff in Hnolevel. destruct_and!.
-      pose proof (IH1 := IHϕ1 level).
-      destruct IH1 as [IH11 _].
-      specialize (IH11 ltac:(assumption) ltac:(assumption)).
-      pose proof (IH2 := IHϕ2 level).
-      destruct IH2 as [IH21 _].
-      specialize (IH21 ltac:(assumption) ltac:(assumption)).
-      split_and!; assumption.
-    - apply orb_false_iff in Hnolevel. destruct_and!.
-      pose proof (IH1 := IHϕ1 level).
-      destruct IH1 as [_ IH12].
-      specialize (IH12 ltac:(assumption) ltac:(assumption)).
-      pose proof (IH2 := IHϕ2 level).
-      destruct IH2 as [_ IH22].
-      specialize (IH22 ltac:(assumption) ltac:(assumption)).
-      split_and!; assumption.
-    - apply orb_false_iff in Hnolevel. destruct_and!.
-      pose proof (IH1 := IHϕ1 level).
-      destruct IH1 as [_ IH12].
-      specialize (IH12 ltac:(assumption) ltac:(assumption)).
-      pose proof (IH2 := IHϕ2 level).
-      destruct IH2 as [IH21 _].
-      specialize (IH21 ltac:(assumption) ltac:(assumption)).
-      split_and!; assumption.
-    - apply orb_false_iff in Hnolevel. destruct_and!.
-      pose proof (IH1 := IHϕ1 level).
-      destruct IH1 as [IH11 _].
-      specialize (IH11 ltac:(assumption) ltac:(assumption)).
-      pose proof (IH2 := IHϕ2 level).
-      destruct IH2 as [_ IH22].
-      specialize (IH22 ltac:(assumption) ltac:(assumption)).
-      split_and!; assumption.
-    - firstorder.
-    - firstorder.
-    - firstorder.
-    - firstorder.
-  Qed.
-
-  Lemma no_negative_occurrence_svar_quantify ϕ level X:
-    no_negative_occurrence_db_b level ϕ = true ->
-    svar_has_negative_occurrence X ϕ = false ->
-    no_negative_occurrence_db_b level (ϕ^{{svar: X ↦ level}}) = true.
-  Proof.
-    intros H1 H2.
-    pose proof (Htmp :=Private_no_negative_occurrence_svar_quantify ϕ level X).
-    destruct Htmp as [Htmp1 Htmp2].
-    auto.
-  Qed.
-
-  Lemma no_positive_occurrence_svar_quantify ϕ level X:
-      no_positive_occurrence_db_b level ϕ = true ->
-      svar_has_positive_occurrence X ϕ = false ->
-      no_positive_occurrence_db_b level (ϕ^{{svar: X ↦ level}}) = true.
-  Proof.
-    intros H1 H2.
-    pose proof (Htmp :=Private_no_negative_occurrence_svar_quantify ϕ level X).
-    destruct Htmp as [Htmp1 Htmp2].
-    auto.
-  Qed.
-
-
-  Lemma no_negative_occurrence_svar_quantify_2 X dbi1 dbi2 ϕ:
-    dbi1 <> dbi2 ->
-    no_negative_occurrence_db_b dbi1 (ϕ^{{svar: X ↦ dbi2}}) = no_negative_occurrence_db_b dbi1 ϕ
-  with no_positive_occurrence_svar_quantify_2  X dbi1 dbi2 ϕ:
-    dbi1 <> dbi2 ->
-    no_positive_occurrence_db_b dbi1 (ϕ^{{svar: X ↦ dbi2}}) = no_positive_occurrence_db_b dbi1 ϕ.
-  Proof.
-    - move: dbi1 dbi2.
-      induction ϕ; intros dbi1 dbi2 Hdbi; simpl; auto.
-      + case_match; reflexivity.
-      + cbn. rewrite IHϕ1. lia. rewrite IHϕ2. lia. reflexivity.
-      + unfold no_negative_occurrence_db_b at 1.
-        fold (no_positive_occurrence_db_b dbi1 (ϕ1^{{svar: X ↦ dbi2}})).
-        fold (no_negative_occurrence_db_b dbi1 (ϕ2^{{svar: X ↦ dbi2}})).
-        rewrite no_positive_occurrence_svar_quantify_2. lia. rewrite IHϕ2. lia. reflexivity.
-      + cbn. rewrite IHϕ. lia. reflexivity.
-      + cbn. rewrite IHϕ. lia. reflexivity.
-    - move: dbi1 dbi2.
-      induction ϕ; intros dbi1 dbi2 Hdbi; simpl; auto.
-      + case_match; cbn. 2: reflexivity. case_match; congruence.
-      + cbn. rewrite IHϕ1. lia. rewrite IHϕ2. lia. reflexivity.
-      + unfold no_positive_occurrence_db_b at 1.
-        fold (no_negative_occurrence_db_b dbi1 (ϕ1^{{svar: X ↦ dbi2}})).
-        fold (no_positive_occurrence_db_b dbi1 (ϕ2^{{svar: X ↦ dbi2}})).
-        rewrite no_negative_occurrence_svar_quantify_2. lia. rewrite IHϕ2. lia. reflexivity.
-      + cbn. rewrite IHϕ. lia. reflexivity.
-      + cbn. rewrite IHϕ. lia. reflexivity.
-  Qed.
-
-  Lemma well_formed_positive_svar_quantify X dbi ϕ:
-    well_formed_positive ϕ ->
-    well_formed_positive (ϕ^{{svar: X ↦ dbi}}) = true.
-  Proof.
-    intros Hϕ.
-    move: dbi.
-    induction ϕ; intros dbi; simpl; auto.
-    - case_match; reflexivity.
-    - simpl in Hϕ.
-      destruct_and!.
-      specialize (IHϕ1 ltac:(assumption)).
-      specialize (IHϕ2 ltac:(assumption)).
-      rewrite IHϕ1. rewrite IHϕ2.
-      reflexivity.
-    - simpl in Hϕ.
-      destruct_and!.
-      specialize (IHϕ1 ltac:(assumption)).
-      specialize (IHϕ2 ltac:(assumption)).
-      rewrite IHϕ1. rewrite IHϕ2.
-      reflexivity.
-    - simpl in Hϕ.
-      destruct_and!.
-      specialize (IHϕ ltac:(assumption)).
-      rewrite IHϕ.
-      rewrite no_negative_occurrence_svar_quantify_2. lia.
-      split_and!; auto.
-  Qed.
-
-  (* Lemma bevar_occur_positivity ψ dbi :
-    bsvar_occur ψ dbi = false ->
-    no_negative_occurrence_db_b dbi ψ = true /\ no_positive_occurrence_db_b dbi ψ.
-  Proof.
-    induction ψ; intros H; cbn; auto.
-    * simpl in H. case_match; auto.
-    * *)
-
-  Lemma nno_free_svar_subst dbi ϕ ψ X:
-    well_formed_closed_mu_aux ψ dbi ->
-    no_negative_occurrence_db_b dbi (ϕ^[[svar: X ↦ ψ]])
-    = no_negative_occurrence_db_b dbi ϕ
-  with npo_free_svar_subst dbi ϕ ψ X:
-    well_formed_closed_mu_aux ψ dbi ->
-    no_positive_occurrence_db_b dbi (ϕ^[[svar: X ↦ ψ]])
-    = no_positive_occurrence_db_b dbi ϕ.
-  Proof.
-    - move: dbi.
-      induction ϕ; intros dbi Hwf; simpl; auto.
-      + case_match; cbn; [|reflexivity].
-        eapply Private_wfc_impl_no_neg_pos_occ. exact Hwf. lia.
-      + cbn. rewrite IHϕ1; auto. rewrite IHϕ2; auto.
-      + cbn.
-        fold (no_positive_occurrence_db_b).
-        rewrite nno_free_svar_subst; auto.
-        rewrite npo_free_svar_subst; auto.
-      + cbn.
-        rewrite IHϕ; auto.
-      + cbn.
-        rewrite IHϕ; auto. eapply well_formed_closed_mu_aux_ind. 2: exact Hwf. lia.
-    - move: dbi.
-      induction ϕ; intros dbi Hwf; simpl; auto.
-      + case_match; cbn; [|reflexivity].
-        eapply Private_wfc_impl_no_neg_pos_occ. exact Hwf. lia.
-      + cbn. rewrite IHϕ1; auto. rewrite IHϕ2; auto.
-      + cbn.
-        fold (no_negative_occurrence_db_b).
-        rewrite nno_free_svar_subst; auto.
-        rewrite IHϕ2; auto.
-      + cbn.
-        rewrite IHϕ; auto.
-      + cbn.
-        rewrite IHϕ; auto. eapply well_formed_closed_mu_aux_ind. 2: exact Hwf. lia.
-  Qed.
-
-  Lemma wfp_free_svar_subst_1 ϕ ψ X:
-    well_formed_closed ψ = true ->
-    well_formed_positive ψ = true ->
-    well_formed_positive ϕ = true ->
-    well_formed_positive (ϕ^[[svar: X ↦ ψ]]) = true.
-  Proof.
-    intros wfcψ wfpψ wfpϕ.
-    induction ϕ; simpl; auto.
-    - case_match; auto.
-    - simpl in wfpϕ. destruct_and!.
-      rewrite -> IHϕ1 by assumption.
-      rewrite -> IHϕ2 by assumption.
-      reflexivity.
-    - simpl in wfpϕ. destruct_and!.
-      rewrite -> IHϕ1 by assumption.
-      rewrite -> IHϕ2 by assumption.
-      reflexivity.
-    - simpl in wfpϕ. destruct_and!.
-      specialize (IHϕ H0).
-      rewrite -> IHϕ.
-      rewrite nno_free_svar_subst.
-      { apply andb_true_iff in wfcψ. apply wfcψ. }
-      rewrite H.
-      reflexivity.
-  Qed.
-
-  Lemma wfp_free_svar_subst ϕ ψ X:
+   Lemma wfp_free_svar_subst ϕ ψ X:
     well_formed_closed_mu_aux ψ 0 ->
     well_formed_positive ψ = true ->
     well_formed_positive ϕ = true ->
@@ -1058,12 +852,22 @@ Section with_signature.
     well_formed (patt_mu ϕ) ->
     well_formed (ϕ^{svar: 0 ↦ X}).
   Proof.
-    intros H. wf_auto;
+    intros H. (*compoundDecomposeWfGoal.
+    apply (unary_wfxy_compose _).*) wf_auto2.
+    (*
+    wf_auto2_fast_done.
+    compositeSimplifyAllWfHyps.
+    wf_auto2_composite_step.
+    wf_auto2_composite_step.
+    Set Printing All.
+    Search well_formed svar_open.
+    wf_auto2.
     destruct_and!;
         [ (apply wfp_svar_open; auto)
         | (apply wfc_mu_aux_body_mu_imp1; assumption)
         | (apply wfc_ex_aux_body_mu_imp1; assumption)
         ].
+    *)
   Qed.
 
 
@@ -1073,7 +877,7 @@ Section with_signature.
   Proof.
     intros Hsubst.
     move: dbi Hsubst.
-    induction ϕ; intros dbi Hsubst; simpl in *; auto.
+    induction ϕ; intros dbi Hsubst; simpl in *; try reflexivity; auto with nocore.
     - apply andb_prop in Hsubst. destruct Hsubst as [Hsubst1 Hsubst2].
       specialize (IHϕ1 dbi Hsubst1).
       specialize (IHϕ2 dbi Hsubst2).
@@ -1092,7 +896,7 @@ Section with_signature.
   Proof.
     intros Hsubst.
     move: dbi Hsubst.
-    induction ϕ; intros dbi Hsubst; simpl in *; auto.
+    induction ϕ; intros dbi Hsubst; simpl in *; try reflexivity; auto with nocore.
     - apply andb_prop in Hsubst. destruct Hsubst as [Hsubst1 Hsubst2].
       specialize (IHϕ1 dbi Hsubst1).
       specialize (IHϕ2 dbi Hsubst2).
@@ -1113,7 +917,7 @@ Section with_signature.
     no_positive_occurrence_db_b dbi ϕ = true.
   Proof.
     - move: dbi.
-      induction ϕ; intros dbi Hsubst; cbn in *; auto.
+      induction ϕ; intros dbi Hsubst; cbn in *; try reflexivity; auto with nocore.
       + apply andb_prop in Hsubst. destruct Hsubst as [Hsubst1 Hsubst2].
         specialize (IHϕ1 dbi Hsubst1).
         specialize (IHϕ2 dbi Hsubst2).
@@ -1127,7 +931,7 @@ Section with_signature.
         erewrite npo_after_subst_impl_npo_before.
         reflexivity. eassumption.
     - move: dbi.
-      induction ϕ; intros dbi Hsubst; cbn in *; auto.
+      induction ϕ; intros dbi Hsubst; cbn in *; try reflexivity; auto with nocore.
       + apply andb_prop in Hsubst. destruct Hsubst as [Hsubst1 Hsubst2].
         specialize (IHϕ1 dbi Hsubst1).
         specialize (IHϕ2 dbi Hsubst2).
@@ -1148,7 +952,7 @@ Section with_signature.
   Proof.
     intros Hsubst.
     move: Hsubst.
-    induction ϕ; intros Hsubst; simpl in *; auto.
+    induction ϕ; intros Hsubst; simpl in *; try reflexivity; auto with nocore.
     - apply andb_prop in Hsubst. destruct Hsubst as [Hsubst1 Hsubst2].
       specialize (IHϕ1 Hsubst1).
       specialize (IHϕ2 Hsubst2).
@@ -1226,123 +1030,6 @@ Section with_signature.
     intros p.
     apply svar_is_fresh_in_dec.
   Defined.
-
-  Lemma no_neg_occ_quan_impl_no_neg_occ x n1 n2 ϕ:
-   no_negative_occurrence_db_b n1 (ϕ^{{evar: x ↦ n2}}) = true ->
-   no_negative_occurrence_db_b n1 ϕ = true
-  with no_pos_occ_quan_impl_no_pos_occ x n1 n2 ϕ:
-   no_positive_occurrence_db_b n1 (ϕ^{{evar: x ↦ n2}}) = true ->
-   no_positive_occurrence_db_b n1 ϕ = true.
-  Proof.
-   - intros H.
-     move: n1 n2 H.
-     induction ϕ; intros n1 n2 H; simpl in *; auto.
-     + unfold no_negative_occurrence_db_b in *. simpl in *. fold no_negative_occurrence_db_b in *.
-       destruct_and!.
-       erewrite -> IHϕ1 by eassumption.
-       erewrite -> IHϕ2 by eassumption.
-       reflexivity.
-     + unfold no_negative_occurrence_db_b in *. simpl in *.
-       fold no_negative_occurrence_db_b no_positive_occurrence_db_b in *.
-       destruct_and!.
-       erewrite -> no_pos_occ_quan_impl_no_pos_occ by eassumption.
-       erewrite -> IHϕ2 by eassumption.
-       reflexivity.
-     + unfold no_negative_occurrence_db_b in *. simpl in *. fold no_negative_occurrence_db_b in *.
-       erewrite -> IHϕ by eassumption.
-       reflexivity.
-     + unfold no_negative_occurrence_db_b in *. simpl in *. fold no_negative_occurrence_db_b in *.
-       erewrite -> IHϕ by eassumption.
-       reflexivity.
-   - intros H.
-     move: n1 n2 H.
-     induction ϕ; intros n1 n2 H; simpl in *; auto.
-     + unfold no_positive_occurrence_db_b in *. simpl in *. fold no_positive_occurrence_db_b in *.
-       destruct_and!.
-       erewrite -> IHϕ1 by eassumption.
-       erewrite -> IHϕ2 by eassumption.
-       reflexivity.
-     + unfold no_positive_occurrence_db_b in *. simpl in *.
-       fold no_positive_occurrence_db_b no_negative_occurrence_db_b in *.
-       destruct_and!.
-       erewrite -> no_neg_occ_quan_impl_no_neg_occ by eassumption.
-       erewrite -> IHϕ2 by eassumption.
-       reflexivity.
-     + unfold no_positive_occurrence_db_b in *. simpl in *. fold no_positive_occurrence_db_b in *.
-       erewrite -> IHϕ by eassumption.
-       reflexivity.
-     + unfold no_positive_occurrence_db_b in *. simpl in *. fold no_positive_occurrence_db_b in *.
-       erewrite -> IHϕ by eassumption.
-       reflexivity.
-  Qed.
-
-  Lemma wfp_evar_quan_impl_wfp x n ϕ:
-    well_formed_positive (ϕ^{{evar: x ↦ n}}) = true ->
-    well_formed_positive ϕ.
-  Proof.
-    intros H.
-    move: n H.
-    induction ϕ; intros n' H; simpl in *; auto.
-    - destruct_and!.
-      erewrite -> IHϕ1 by eassumption.
-      erewrite -> IHϕ2 by eassumption.
-      reflexivity.
-    - destruct_and!.
-      erewrite -> IHϕ1 by eassumption.
-      erewrite -> IHϕ2 by eassumption.
-      reflexivity.
-    - erewrite IHϕ by eassumption.
-      reflexivity.
-    - simpl.
-      destruct_and!.
-      erewrite -> IHϕ by eassumption.
-      erewrite -> no_neg_occ_quan_impl_no_neg_occ by eassumption.
-      reflexivity.
-  Qed.
-
-  Lemma wfcex_evar_quan_impl_wfcex x n dbi ϕ:
-    well_formed_closed_ex_aux (ϕ^{{evar: x ↦ n}}) dbi = true ->
-    well_formed_closed_ex_aux ϕ dbi.
-  Proof.
-    intros H.
-    move: n dbi H.
-    induction ϕ; intros n' dbi H; simpl in *; auto.
-    - destruct_and!.
-      erewrite -> IHϕ1 by eassumption.
-      erewrite -> IHϕ2 by eassumption.
-      reflexivity.
-    - destruct_and!.
-      erewrite -> IHϕ1 by eassumption.
-      erewrite -> IHϕ2 by eassumption.
-      reflexivity.
-    - erewrite IHϕ by eassumption.
-      reflexivity.
-    - simpl.
-      erewrite -> IHϕ by eassumption.
-      reflexivity.
-  Qed.
-
-  Lemma wfcmu_evar_quan_impl_wfcmu x n dbi ϕ:
-    well_formed_closed_mu_aux (ϕ^{{evar: x ↦ n}}) dbi = true ->
-    well_formed_closed_mu_aux ϕ dbi.
-  Proof.
-    intros H.
-    move: n dbi H.
-    induction ϕ; intros n' dbi H; simpl in *; auto.
-    - destruct_and!.
-      erewrite -> IHϕ1 by eassumption.
-      erewrite -> IHϕ2 by eassumption.
-      reflexivity.
-    - destruct_and!.
-      erewrite -> IHϕ1 by eassumption.
-      erewrite -> IHϕ2 by eassumption.
-      reflexivity.
-    - erewrite IHϕ by eassumption.
-      reflexivity.
-    - simpl.
-      erewrite -> IHϕ by eassumption.
-      reflexivity.
-  Qed.
 
   Lemma wfc_ex_lower ϕ n:
     bevar_occur ϕ n = false ->
