matching-logic/src/wftactics.v
@@ -1,7 +1,15 @@
+From LibHyps Require Import LibHyps.
+
 From Coq Require Import ssreflect ssrfun ssrbool.
+
+From Ltac2 Require Import Ltac2.
+
+From Coq Require Import Btauto.
 
 From stdpp Require Import countable infinite.
 From stdpp Require Import pmap gmap mapset fin_sets propset.
+
+
 Require Import stdpp_ext.
 
 From MatchingLogic
@@ -14,166 +22,402 @@ Require Import
   SyntacticConstruct
 .
 
+Set Default Proof Mode "Classic".
 
-Tactic Notation "wf_auto" int_or_var(n)
-  := auto n; unfold well_formed, well_formed_closed in *; destruct_and?; simpl in *; split_and?; auto n.
-Tactic Notation "wf_auto" := wf_auto 5.
 
-Ltac wf_auto2 := unfold is_true in *;
-repeat (try assumption; try reflexivity; try (solve [wf_auto]); (* TODO: get rid of [wf_auto] *)
-apply nullary_wf || apply unary_wf || apply binary_wf ||
-match goal with
-| [ |- (forall _, _) ]
-  => intro
+(* This hook is specifically intended to be filled with a tactic which
+   transforms provability hypotheses into well_formedness hypotheses.
+   We call it early, before any goal splitting is done,
+   so that it is not called for all the subgoals again and again.
+ *)
+ Ltac2 mutable proved_hook_wfauto
+ := (fun () => () (* Message.print (Message.of_string "hook_wfauto base") *)).
+ 
+ (* We give a name to the wrapper so that it is shown in the profile (when profiling). *)
+ Ltac proved_hook_wfauto := ltac2:(|- proved_hook_wfauto ()).
+ 
 
-| [ |- size' (evar_open _ _ _) < _ ]
-  => rewrite evar_open_size'
-
-| [ |- size' (svar_open _ _ _) < _ ]
-  => rewrite svar_open_size'
-
-| [ |- size' _ < size' (patt_app _ _) ]
-  => simpl; lia
-
-| [ |- size' _ < size' (patt_imp _ _) ]
-  => simpl; lia
-
-| [ |- size' _ < size' (patt_exists _) ]
-  => simpl; lia
-
-| [ |- well_formed (foldr patt_imp ?g ?xs) = true ]
-  => apply well_formed_foldr
-
-| [ |- wf (take ?n ?xs) = true ]
-  => apply wf_take
-
-| [ |- wf (drop ?n ?xs) = true ]
-  => apply wf_drop
-
-| [ |- wf (<[?n := ?p]> ?xs) = true ]
-  => apply wf_insert
-
-| [ |- wf (?x :: ?xs) = true ]
-  => apply wf_cons
-
-| [ |- wf (?xs ++ ?ys) = true ]
-  => apply wf_app
-
-| [ |- well_formed (patt_free_evar _) = true]
-  => reflexivity
-
-| [ |- well_formed (patt_free_svar _) = true]
-  => reflexivity
-
-| [ H : well_formed (patt_app ?p ?q) = true |- _]
-  => assert (well_formed p = true);
-    [eapply well_formed_app_proj1; eassumption|];
-    assert ( well_formed q = true);
-    [eapply well_formed_app_proj2; eassumption|];
-    clear H
-
-| [ H : well_formed (patt_imp ?p ?q) = true |- _]
-  => assert (well_formed p = true);
-    [eapply well_formed_imp_proj1; eassumption|];
-    assert ( well_formed q = true);
-    [eapply well_formed_imp_proj2; eassumption|];
-    clear H
-
-| [ |- well_formed (free_evar_subst ?phi ?p ?E) = true ]
-  => apply well_formed_free_evar_subst
-
-| [ |- ?x ∉ ?E ]
-  => progress simpl
-
-| [ |- ?x ∉ free_evars (free_evar_subst _ _ _) ]
-  => eapply not_elem_of_larger_impl_not_elem_of;
-     [apply free_evars_free_evar_subst|]
-
-| [frx: ?x ∉ _ |- ?x <> ?E ]
-  => clear -frx; set_solver
-
-| [frx: ?x ∉ _ |- ?x ∉ ?E ]
-  => clear -frx; set_solver
-
-| [ |- well_formed (evar_open _ _ _) = true]
-  => apply wf_evar_open_from_wf_ex
-
-| [ |- well_formed (@subst_ctx _ _ _) = true]
-  => apply wf_sctx
-
-  (* fallback *)
-| [ |- well_formed _ = true]
-  => unfold well_formed, well_formed_closed in *; simpl in *;
-     destruct_and?; split_and?
-
-| [ |- well_formed_positive (free_evar_subst _ _ _) = true ]
-  => apply wfp_free_evar_subst
-
-| [H: well_formed_positive (patt_exists _) = true |- _]
-  => simpl in H
-
-| [H: well_formed_closed_mu_aux (patt_exists _) _ = true |- _]
-  => simpl in H
-
-| [H: well_formed_closed_ex_aux (patt_exists _) _ = true |- _]
-  => simpl in H
-
-| [ |- well_formed_closed_mu_aux (free_evar_subst _ _ _) _ = true]
-  => apply wfc_mu_free_evar_subst
-
-| [ |- well_formed_closed_ex_aux (free_evar_subst _ _ _) _ = true]
-  => apply wfc_ex_free_evar_subst_2; simpl
-
-| [ |- well_formed_positive (bsvar_subst _ _ _) = true ]
-  => apply wfp_bsvar_subst
-
-| [ |- well_formed_positive _ = true ]
-  => progress (simpl; split_and?)
-
-| [ |- no_negative_occurrence_db_b _ (free_evar_subst _ _ _) = true ]
-  => apply free_evar_subst_preserves_no_negative_occurrence
-
-| [ |- well_formed_closed_mu_aux (bsvar_subst _ _ _) _ = true ]
-  => apply wfc_mu_aux_bsvar_subst
-
-| [ |- well_formed_closed_ex_aux (bsvar_subst _ _ _) _ = true ]
-  => apply wfc_ex_aux_bsvar_subst
-
-| [ |- svar_has_negative_occurrence _ (svar_open _ _ _) = false] =>
-  unfold svar_open; apply svar_hno_bsvar_subst
-
-|[ |- context C [ svar_quantify _ _ (svar_open _ _ _) ] ]
-  => rewrite svar_quantify_svar_open
-
-| [ |- well_formed_closed_mu_aux (svar_open _ _ _) _ = true] =>
-  unfold svar_open; apply wfc_mu_aux_bsvar_subst
-
-| [ |- well_formed_closed_ex_aux (svar_open _ _ _) _ = true] =>
-  unfold svar_open; apply wfc_ex_aux_bsvar_subst
-
-| [ |- no_negative_occurrence_db_b _ _ = true ]
-  => solve [unfold well_formed in *; simpl in *; destruct_and!; assumption]
-
-| [ |- no_negative_occurrence_db_b _ (free_evar_subst _ _ _) = true ]
-  => apply free_evar_subst_preserves_no_negative_occurrence
-
-(* last option for [svar_has_negative_occurrence] *)
-| [ |- svar_has_negative_occurrence _ _ = false ]
-  => apply svar_hno_false_if_fresh
-
-| [ |- svar_is_fresh_in _ _ ]
-  => unfold svar_is_fresh_in
-
-  (* last option for well_formed_closed_ex_aux: try decreasing n *)
-| [ |- well_formed_closed_ex_aux ?p (S ?n) = true ]
-  => eapply well_formed_closed_ex_aux_ind with (ind_evar1 := n);[lia|]
-
-  (* last option for well_formed_closed_mu_aux: try decreasing n *)
-| [ |- well_formed_closed_mu_aux ?p (S ?n) = true ]
-  => eapply well_formed_closed_mu_aux_ind with (ind_svar1 := n);[lia|]
-
-end; unfold is_true in *
+Definition wfToWfxySimplifications := (
+  @wf_wfxy00,
+  @wf_lwf_xy
 ).
+
+Definition wfxySimplifications := (
+  @binary_wfxy,
+  @unary_wfxy,
+  @nullary_wfxy,
+  @lwf_xy_app,
+  @lwf_xy_cons,
+  @well_formed_xy_foldr_binary
+).
+
+Ltac simplifyWfxyHyp H :=
+  unfold is_true in H;
+  lazymatch type of H with
+  | well_formed _ = true
+    => apply wf_wfxy00_decompose in H
+  | Pattern.wf _ = true
+    => apply wf_lwf_xy_decompose in H
+  | _ => idtac
+  end;
+  try lazymatch type of H with
+  | well_formed_xy ?m ?n (foldr ?binary ?g ?xs) = true
+    => apply (well_formed_xy_foldr_binary_decompose _) in H;
+       let H1 := fresh "H1" in
+       let H2 := fresh "H2" in
+       destruct H as [H1 H2];
+       simplifyWfxyHyp H1;
+       simplifyWfxyHyp H2
+  | lwf_xy ?m ?n (?x::?xs) = true
+    => apply lwf_xy_cons_decompose in H;
+       let H1 := fresh "H1" in
+       let H2 := fresh "H2" in
+       destruct H as [H1 H2];
+       simplifyWfxyHyp H1;
+       simplifyWfxyHyp H2
+  | lwf_xy ?m ?n (?xs ++ ?ys) = true
+    => apply lwf_xy_app_decompose in H;
+      let H1 := fresh "H1" in
+      let H2 := fresh "H2" in
+      destruct H as [H1 H2];
+      simplifyWfxyHyp H1;
+      simplifyWfxyHyp H2
+  | well_formed_xy ?x ?y (?binary ?ψ1 ?ψ2) = true
+    => apply (binary_wfxy_decompose _) in H;
+      let H1 := fresh "H1" in
+      let H2 := fresh "H2" in
+      destruct H as [H1 H2];
+      simplifyWfxyHyp H1;
+      simplifyWfxyHyp H2
+  | well_formed_xy ?x ?y (?unary ?ψ1) = true
+    => apply (unary_wfxy_decompose _) in H;
+       simplifyWfxyHyp H
+  (* No point in simplifying these *)
+  (*
+  | well_formed_xy ?x ?y ?nullary = true
+    => apply nullary_wfxy in H
+    *)
+  | _ => idtac
+  end
+.
+
+Ltac compositeSimplifyAllWfHyps :=
+  (*proved_hook_wfauto;*)
+  (onAllHyps simplifyWfxyHyp)
+.
+
+
+Ltac compoundDecomposeWfGoal :=
+  rewrite ?wfToWfxySimplifications;
+  rewrite ?wfxySimplifications;
+  lazymatch goal with
+  | [ |- ?g] =>
+    split_and?;
+    lazymatch goal with
+    | [ |- ?g'] => idtac (*"Goal " g' " from " g "."*)
+    end
+  end
+.
+
+
+Ltac propagateTrueInHyps :=
+  repeat (
+    match goal with
+    | [H: _ |- _] => (
+        rewrite !(andb_true_r,andb_true_l) in H
+      )
+    end
+  )
+.
+
+Ltac propagateTrueInGoal :=
+  rewrite !(andb_true_r,andb_true_l)
+.
+
+Ltac clear_all_impls :=
+  repeat (
+    match goal with
+    | [ H : forall _, _ |- _] => clear H
+    end
+  ).
+
+
+  Ltac wf_auto2_decompose_hyps :=
+    proved_hook_wfauto;
+    unfold
+      is_true,
+      evar_open,
+      svar_open
+    in *;
+    simpl in *
+  .
+  
+
+Ltac solve_size :=
+  repeat (
+  match goal with
+  | [ |- size' (evar_open _ _ _) < _ ]
+    => rewrite evar_open_size'
+
+  | [ |- size' (svar_open _ _ _) < _ ]
+    => rewrite svar_open_size'
+
+  | [ |- size' _ < size' (patt_app _ _) ]
+    => simpl; lia
+
+  | [ |- size' _ < size' (patt_imp _ _) ]
+    => simpl; lia
+
+  | [ |- size' _ < size' (patt_exists _) ]
+    => simpl; lia
+  end
+  )
+.
+Ltac wf_auto2_fast_done :=
+  try solve_size;
+  try assumption;
+  try reflexivity;
+  try congruence;
+  try btauto
+.
+  
+Ltac wf_auto2_composite_step :=
+  unfold is_true;
+  simpl;
+  first [
+    split |
+    apply wf_wfxy00_compose |
+    apply wf_lwf_xy_compose |
+    apply free_evar_subst_preserves_no_negative_occurrence |
+    apply wf_sctx |
+    apply well_formed_xy_free_evar_subst |
+    apply (well_formed_xy_foldr_binary_compose _) |
+    apply lwf_xy_cons_compose |
+    apply lwf_xy_app_compose |
+    apply (binary_wfxy_compose _) |
+    apply (unary_wfxy_compose _) |
+    apply (nullary_wfxy _) |
+    apply wf_evar_open_from_wf_ex |
+    apply wf_sctx
+  ];
+  wf_auto2_fast_done
+  (*compoundDecomposeWfGoal*)
+.
+
+Definition wfPositiveSimplifications := (
+  @well_formed_positive_foldr_binary,
+  @nullary_wfp,
+  @unary_wfp,
+  @binary_wfp,
+  @wfp_evar_quan
+).
+
+Definition wfCexSimplifications := (
+  @well_formed_cex_foldr_binary,
+  @nullary_wfcex,
+  @unary_wfcex,
+  @binary_wfcex
+).
+
+Definition wfCmuSimplifications := (
+  @well_formed_cmu_foldr_binary,
+  @nullary_wfcmu,
+  @unary_wfcmu,
+  @binary_wfcmu,
+  @wfcmu_evar_quan
+).
+
+Definition wfSimplifications := (
+  @wf_corr,
+  @andb_true_r
+).
+
+Definition lwfPositiveSimplifications := (
+  @lwf_positive_cons,
+  @lwf_positive_app
+).
+
+Definition lwfCmuSimplifications := (
+  @lwf_cmu_cons,
+  @lwf_cmu_app
+).
+
+Definition lwfCexSimplifications := (
+  @lwf_cex_cons,
+  @lwf_cex_app
+).
+
+Ltac partsDecomposeWfGoal :=
+  rewrite -?wfxy00_wf;
+  rewrite !(wfPositiveSimplifications,
+            wfCexSimplifications,
+            wfCmuSimplifications,
+            wfSimplifications,
+            lwfPositiveSimplifications,
+            lwfCmuSimplifications,
+            lwfCexSimplifications,
+            lwf_xy_decompose)
+.
+
+
+Ltac simplifyWfHypParts H :=
+  let t := type of H in
+  (* idtac "SimplifyWfHypParts " H " (" t ")"; *)
+  lazymatch type of H with
+  | well_formed_positive _ = true
+    =>
+      rewrite ?wfPositiveSimplifications in H;
+      destruct_andb? H
+  (* We are doing lazymatch, so this has to be before the general case*)
+  | well_formed_closed_ex_aux (bevar_subst (patt_free_evar ?x) ?k ?p) ?k = true
+      =>
+        apply wfc_ex_aux_S_bevar_subst_fe in H
+  | well_formed_closed_ex_aux _ _ = true
+    =>
+      rewrite ?wfCexSimplifications in H;
+      destruct_andb? H
+  | well_formed_closed_mu_aux _ _ = true
+    =>
+      rewrite ?wfCmuSimplifications in H;
+      destruct_andb? H
+  | Pattern.wf _ = true
+    =>
+      rewrite wf_corr in H;
+      destruct_andb? H
+  | lwf_positive _ = true
+    =>
+      rewrite ?lwfPositiveSimplifications in H;
+      destruct_andb? H
+  | lwf_cmu _ _ = true
+    =>
+      rewrite ?lwfCmuSimplifications in H;
+      destruct_andb? H
+  | lwf_cex _ _ = true
+    =>
+      rewrite ?lwfCexSimplifications in H;
+      destruct_andb? H
+  | lwf_xy _ _ _ = true
+    =>
+      rewrite lwf_xy_decompose in H;
+      destruct_andb? H
+  | _ => idtac
+  end
+.
+
+Ltac toBeRunOnAllHypsParts h := simplifyWfHypParts h.
+
+Ltac simplifyAllWfHypsParts :=
+  (onAllHyps toBeRunOnAllHypsParts) ;{ toBeRunOnAllHypsParts }
+.
+
+
+Ltac decomposeWfHypsIntoParts :=
+  simplifyAllWfHypsParts
+.
+
+
+Ltac wf_auto2_unfolds :=
+  unfold
+    is_true,
+    well_formed,
+    well_formed_closed,
+    well_formed_xy,
+    evar_open,
+    svar_open(*,
+    free_evar_subst,
+    free_evar_subst*)
+  in *
+.
+
+Ltac wf_auto2_decompose_hyps_parts :=
+  proved_hook_wfauto;
+  wf_auto2_unfolds;
+  simpl in *;
+  destruct_andb?;
+  decomposeWfHypsIntoParts
+.
+
+Ltac wf_auto2_step_parts :=
+  wf_auto2_unfolds;
+  try partsDecomposeWfGoal;
+  cbn in *; subst; cbn in *;
+  split_and?;
+  wf_auto2_fast_done;
+  try lazymatch goal with
+  | [MF : mu_free ?p = true |- well_formed_positive (bevar_subst _ _ ?p) = true]
+    => apply bevar_subst_positive; solve wf_auto2_step_parts
+  end;
+  try first [
+  apply wfp_free_evar_subst |
+  apply wfc_ex_free_evar_subst_2 |
+  apply wfc_mu_free_evar_subst |
+  apply svar_hno_bsvar_subst |
+  apply svar_hno_false_if_fresh |
+  apply well_formed_positive_svar_quantify |
+  apply free_evar_subst_preserves_no_negative_occurrence |
+  apply no_negative_occurrence_svar_quantify |
+  apply bevar_subst_closed_mu|
+  apply bevar_subst_closed_ex|
+  apply bevar_subst_positive_2|
+  apply evar_quantify_closed_ex|
+  apply svar_quantify_closed_ex|
+  apply evar_quantify_closed_mu|
+  apply svar_quantify_closed_mu|
+  apply wfp_free_svar_subst_1|
+  apply wfc_mu_free_svar_subst|
+  apply wfc_ex_free_svar_subst|
+  apply wp_sctx|
+  apply wcmu_sctx|
+  apply wcex_sctx|
+  apply wfp_bsvar_subst|
+  apply wfc_mu_aux_bsvar_subst|
+  apply wfc_ex_aux_bsvar_subst
+  ];
+  try (lazymatch goal with
+  | [ H : well_formed_closed_mu_aux ?p 0 = true |- no_negative_occurrence_db_b _ ?p = true]
+    => apply wfc_impl_no_neg_occ; apply H
+
+  | [ H : well_formed_closed_mu_aux ?p 0 = true |- no_positive_occurrence_db_b _ ?p = true]
+    => apply wfc_impl_no_pos_occ; apply H
+
+  | [ H : well_formed_closed_ex_aux ?p _ = true |- well_formed_closed_ex_aux ?p (S ?n) = true ]
+    => eapply well_formed_closed_ex_aux_ind;[|apply H]; lia
+
+    (* last option for well_formed_closed_mu_aux: try decreasing n *)
+  | [ H : well_formed_closed_mu_aux ?p _ = true |- well_formed_closed_mu_aux ?p (S ?n) = true ]
+    => eapply well_formed_closed_mu_aux_ind;[|apply H]; lia
+  end)
+.
+
+Ltac wf_auto2_fast :=
+  wf_auto2_fast_done;
+  compositeSimplifyAllWfHyps;
+  repeat wf_auto2_composite_step
+.
+
+Ltac print_hyps :=
+  try match goal with
+  | [H : ?t |- _] => idtac t; fail
+  end
+.
+
+Ltac wf_auto2_fallback :=
+  match goal with
+  | [ |- ?G ] => idtac "Falling back on " G (*; print_hyps*)
+  end;
+  repeat wf_auto2_decompose_hyps_parts;
+  repeat wf_auto2_step_parts
+.
+
+Ltac wf_auto2 :=
+  try reflexivity; (* this generates a simple proof: just eq_refl*)
+  subst;
+  proved_hook_wfauto;
+  clear_all_impls;
+  (*clear_others;*)
+  wf_auto2_fast;
+  wf_auto2_fallback
+.
 
 Ltac try_wfauto2 :=
 lazymatch goal with
